Logic/Propositional/Superintuitionistic/Kripke/Completeness.lean
@@ -587,7 +587,6 @@ lemma complete (H : CanonicalFrame Λ ∈ 𝔽) {p : Formula α} : 𝔽#α ⊧ p
 instance instComplete (H : CanonicalFrame Λ ∈ 𝔽) : Complete Λ (𝔽#α) := ⟨complete H⟩
 
 instance Int_Complete : Complete (𝐈𝐧𝐭 : DeductionParameter α) (Kripke.ReflexiveTransitiveFrameClass.{u}#α) := instComplete $ by
-  simp;
   constructor;
   . exact CanonicalFrame.reflexive;
   . exact CanonicalFrame.transitive;
